\documentclass{article}
\usepackage{graphicx} % Required for inserting images

\begin{document}

\section*{Problem 3}

\[
    (B - A) \cup (C - A) \;=\; (B \cup C) - A
\]

We can prove that the above equation is true. To start, we can say that on the right side, we are combining sets B and C. We are then removing everything from \[(B \cup C)\], that is within the set of A. This means that we are left with a set of everything in set B that is not in set A plus everything in the set C that is not also in A.

In other words, we are saying that we will end up with a set that contains element from
(B - A) and (C - A)
. In set notation, this would be \[
    (B - A) \cup (C - A)
\]. This means that \[
    (B - A) \cup (C - A) \;=\; (B \cup C) - A
\]

\section*{Example}

Let
\[
    B = \{1,2,3,4\}, \quad C = \{5,6,7,8\}, \quad A = \{1,2,5,6\}.
\]

\textbf{Left-hand side:}
\[
    B - A = \{3,4\}, \quad C - A = \{7,8\}.
\]
Thus,
\[
    (B - A) \cup (C - A) = \{3,4,7,8\}.
\]

\textbf{Right-hand side:}
\[
    B \cup C = \{1,2,3,4,5,6,7,8\},
\]
so
\[
    (B \cup C) - A = \{3,4,7,8\}.
\]

Since both sides equal $\{3,4,7,8\}$, the identity holds in this example.

\end{document}



\end{document}
