\documentclass[11pt]{article}
\usepackage{amsmath}
\usepackage{amssymb}

\begin{document}

\section{Problem 1}

Let $P(n)$ be the proposed statement that $2^{(n-1)} + 2 \cdot 4^{(n-1)}$ is a closed form solution for the recurrence relation for the number of length $n$ codewords you can make if you must have an even number of $0$s. We want to prove that P(n) is true for integers $n \ge 1$. The recurrence relation is defined as 
\[
q_n = 2(q_{n-1}) + 4^{\,n-1}.
\]

Lets look at the proposed statement of $P(1)$:

\[
P(1) = 2^{(1-1)} + 2 \cdot 4^{(1-1)} = 2^0 + 2 \cdot 4^0 = 3.
\]

When looking at the recurrence relation, $q_1$ is equal to $3$. This means that when $n = 1$, the recurrence relation and the proposed closed-form solution are equal.

As our inductive hypothesis, assume that $P(n)$ holds for SOME $k \ge 1$. We will look at the case of $P(k+1)$ and $q_{k+1}$.

\[
q_{k+1} = 2(q_k) + 4^{(k+1)-1}.
\]

Through induction, we say $q_k = P_k$. So:

\[
q_{k+1} = 2(2^{k-1}) + 2(4^{k-1}) + 4^{(k+1)-1}.
\]

With algebra, we can simplify to:

\[
q_{k+1} = 2(2^{k-1}) + 2(4^{k-1}) + 4^k,
\]

\[
q_{k+1} = 2 \cdot 2^{k-1} + 2 \cdot 2(4^{k-1}) + 4^k,
\]

\[
q_{k+1} = 2 \cdot 2^{k-1} + 4(4^{k-1}) + 4^k,
\]

\[
q_{k+1} = 2 \cdot 2^{k-1} + 4^k + 4^k,
\]

\[
q_{k+1} = 2^k + 2 \cdot 4^k,
\]

\[
q_{k+1} = 2^{(k+1)-1} + 2 \cdot 4^{(k+1)-1} = P(k+1).
\]

Since the base case of $P(1)$ holds and since the $(k+1)$st case holds true, $P(n)$ must be true for all positive integers where $n \ge 1$.


\begin{itemize}
    \item \textbf{Who Contributed:} Pranav Bonthu was the main contributor, doing the formal write-up of the solution. Mikey Ku and Dhvan Shah compared their solutions to Pranav's and provided feedback and edits.
    \item \textbf{Resources}: The textbook, class notes
    \item \textbf{Main points:} Based on group discussions, we felt that the main point of this problem was to understand how to prove that the closed form and recurrence relation are equal.
\end{itemize}

\end{document}



